<?xml version="1.0"?>
<rdf:RDF
    xmlns:rdf="http://www.w3.org/1999/02/22-rdf-syntax-ns#"
    xmlns:rdfs="http://www.w3.org/2000/01/rdf-schema#"
    xmlns:rdfa="http://www.w3.org/ns/rdfa#"
    xmlns:owl="http://www.w3.org/2002/07/owl#"
    xmlns:skos="http://www.w3.org/2004/02/skos/core#" 
    xmlns:dc="http://purl.org/dc/elements/1.1/"
    xmlns:dcterms="http://purl.org/dc/terms/"
    xmlns:foaf="http://xmlns.com/foaf/0.1/"
    xmlns:voaf="http://purl.org/vocommons/voaf#"
    xmlns:xsd="http://www.w3.org/2001/XMLSchema#"
    xmlns:metam="http://purl.org/metam#">

    <!-- The Meta Mesh Ontology (MMO) integrates diverse psychiatric knowledge bases into a cohesive framework, enhancing diagnostic precision and personalized treatment. -->
    <!-- It unifies medical, psychological, and social data for a comprehensive understanding of mental health. -->
    <owl:Ontology rdf:about="http://purl.org/htp">
        <rdfs:label>Meta Mesh Ontology</rdfs:label>
        <rdfs:comment>The Meta Mesh Ontology (MMO) is a unified framework designed to integrate diverse knowledge bases in psychiatry, facilitating more accurate and personalized diagnostic and treatment approaches.</rdfs:comment>
        <rdfs:seeAlso rdf:resource="https://www.hitop-system.org/"/>
        <owl:versionInfo>1.3</owl:versionInfo>
        <dc:creator>
            <foaf:Person>
                <foaf:name>Dr. Rogério Blitz</foaf:name>
                <foaf:mbox rdf:resource="mailto:rogerio.blitz@med.uni-jena.de"/>
            </foaf:Person>
        </dc:creator>
        <dc:date>2024-08-21</dc:date>
        <dc:publisher>Dr. Rogério Blitz, Prof. Dr. Nils Opel</dc:publisher>
        <dc:contributor>Prof. Dr. Nils Opel</dc:contributor>
        <dcterms:issued>2024-08-21</dcterms:issued>
        <dcterms:rightsHolder>Dr. Rogério Blitz, Prof. Dr. Nils Opel</dcterms:rightsHolder>
        <dcterms:rightsHolder>Universitätsklinikum Jena</dcterms:rightsHolder>
        <dcterms:license rdf:resource="https://creativecommons.org/licenses/by-nc-nd/4.0/"/>
        <dcterms:rights>This work is licensed under a Creative Commons Attribution-NonCommercial-NoDerivs 4.0 International License.</dcterms:rights>
    </owl:Ontology>

    <!-- Indicates potential future updates to the Meta Mesh Ontology, allowing the inclusion of new knowledge bases and components. -->
    <!-- Highlights the ontology's flexibility to incorporate new elements and relationships as research evolves. -->
    <owl:AnnotationProperty rdf:about="http://purl.org/htp#futureReleaseInfo">
        <rdfs:label>Future Release Information</rdfs:label>
        <rdfs:comment>
            This ontology is designed with flexibility to incorporate new knowledge bases as research and scientific insights evolve. 
            Future updates will facilitate the addition of new elements and relationships, ensuring continuous enhancement and refinement of the ontology.
        </rdfs:comment>
    </owl:AnnotationProperty>

    <!-- Annotation for Thesauri, Taxonomies, and Classification Systems -->
    <!-- This annotation describes the use of SKOS for structured knowledge organization -->
    <owl:AnnotationProperty rdf:about="http://www.w3.org/2004/02/skos/core#">
        <rdfs:label>Thesauri, Taxonomies, and Classification Systems</rdfs:label>
        <rdfs:comment>
        SKOS (Simple Knowledge Organization System) is used for modeling thesauri, taxonomies, and classification systems. 
        It allows the representation of concepts and their hierarchies.
        </rdfs:comment>
    </owl:AnnotationProperty>

    <!-- Annotation for Ontologies -->
    <!-- This annotation describes the use of OWL for defining and managing ontologies -->
    <owl:AnnotationProperty rdf:about="http://www.w3.org/2002/07/owl#">
        <rdfs:label>Ontology</rdfs:label>
        <rdfs:comment>
            OWL (Web Ontology Language) concepts can also be represented in RDF. OWL uses RDF syntax to define ontologies, 
            including classes, properties, and complex relationships. The OWL specification extends RDF and RDFS 
            (RDF Schema), allowing you to use OWL elements such as rdf:Class, rdf:Property, rdfs:subClassOf, and OWL-specific constructs 
            in an RDF file.
        </rdfs:comment>
    </owl:AnnotationProperty>

    <!-- Annotation for Semantic Networks and Knowledge Graphs -->
    <!-- This annotation describes the use of RDF for representing semantic networks and knowledge graphs -->
    <owl:AnnotationProperty rdf:about="http://www.w3.org/1999/02/22-rdf-syntax-ns#">
        <rdfs:label>Semantic Networks and Knowledge Graphs</rdfs:label>
        <rdfs:comment>
            RDF (Resource Description Framework) itself forms the basis for representing semantic networks and knowledge graphs, as it allows 
            relationships between entities to be expressed in a triple format. RDF triples and the use of ontologies 
            enable the modeling of complex knowledge structures.
        </rdfs:comment>
    </owl:AnnotationProperty>

    <!-- Annotation for Rule Systems -->
    <!-- This annotation describes the use of BFO for integrating and managing rule-based systems -->
    <owl:AnnotationProperty rdf:about="http://purl.obolibrary.org/obo/bfo.owl#">
        <rdfs:label>Rule Systems</rdfs:label>
        <rdfs:comment>
            The Basic Formal Ontology (BFO) is suitable for this use case as it provides a top-level ontology framework 
            that can integrate different types of representations, including rule-based systems. BFO facilitates the 
            structuring and categorization of entities and their relations at a very high level of abstraction, which 
            is essential for formalizing rules and ensuring interoperability across various domains and data models. 
            By using BFO, rule systems can be conceptualized within a unified framework that aligns with other knowledge 
            representations, thereby supporting a more coherent and comprehensive approach to ontology-based reasoning 
            and data integration.
        </rdfs:comment>
    </owl:AnnotationProperty>

    <!-- Annotation for Model-Based Representations -->
    <!-- This annotation describes the use of OWL for defining and managing model-based representations -->
    <owl:AnnotationProperty rdf:about="http://www.w3.org/2002/07/owl#">
        <rdfs:label>Model-Based Representations</rdfs:label>
        <rdfs:comment>
            Model-based representations can be captured using OWL classes and properties within RDF. 
            The structure and semantics of models can be expressed through RDF triples and OWL annotations.  
            OWL (Web Ontology Language) is particularly suitable for this use case because it provides a formal semantics 
            that enables precise modeling of complex knowledge structures. OWL extends RDF and RDFS (RDF Schema) with 
            additional ontological constructs such as classes, properties, and restrictions, allowing for the creation 
            of complex models with well-defined relationships and hierarchies. By using OWL, model-based representations 
            can express not only structural, but also logical dependencies and constraints between entities, leading to 
            a richer and more expressive representation. OWL also supports inference mechanisms that enable the generation 
            of new knowledge from existing data, facilitating the analysis and management of complex models.
        </rdfs:comment>
    </owl:AnnotationProperty>

    <!-- Annotation for Corpus-Based Representations -->
    <!-- This annotation describes the use of Dublin Core Terms (dcterms) for metadata and annotations of corpora -->
    <owl:AnnotationProperty rdf:about="http://purl.org/dc/terms/">
        <rdfs:label>Corpus-Based Representations</rdfs:label>
        <rdfs:comment>
            For corpus-based representations, RDF can be used to represent annotations and metadata for corpora. 
            However, RDF does not provide specialized support for processing large text corpora; the corpus data itself 
            would be managed outside the RDF data structure.       
            Dublin Core Terms (dcterms) is particularly suitable for this use case because it provides a set of 
            vocabulary terms that are widely used for describing a wide range of resources, including text corpora. 
            dcterms enables the detailed description of metadata elements such as title, creator, subject, date, and 
            format, which are essential for managing and organizing corpora. By using dcterms within RDF, it is possible 
            to standardize the metadata associated with corpora, ensuring interoperability and facilitating data exchange 
            across different systems. This standardization is crucial for enabling effective search, retrieval, and 
            analysis of corpus data, especially when dealing with large and diverse text collections.
        </rdfs:comment>
    </owl:AnnotationProperty>

    <owl:Class rdf:about="http://purl.org/metam#ClassificationConcept">
        <rdfs:label>Classification Concept</rdfs:label>
        <rdfs:comment></rdfs:comment>
        <rdfs:subClassOf rdf:resource="http://purl.obolibrary.org/obo/bfo.owl#gdc"/>
    </owl:Class>

    <owl:Class rdf:about="http://purl.org/metam#DescriptiveConcept">
        <rdfs:label>Descriptive Concept</rdfs:label>
        <rdfs:comment></rdfs:comment>
        <rdfs:subClassOf rdf:resource="http://purl.obolibrary.org/obo/bfo.owl#sdc"/>
    </owl:Class>

    <owl:Class rdf:about="http://purl.org/metam#PersistentConcept">
        <rdfs:label>Persistent Concept</rdfs:label>
        <rdfs:comment></rdfs:comment>
        <rdfs:subClassOf rdf:resource="http://purl.obolibrary.org/obo/bfo.owl#ic"/>
    </owl:Class>

    <owl:Class rdf:about="http://purl.org/metam#TemporalConcept">
        <rdfs:label>Temporal Concept</rdfs:label>
        <rdfs:comment></rdfs:comment>
        <rdfs:subClassOf rdf:resource="http://purl.obolibrary.org/obo/bfo.owl#occurrent"/>
    </owl:Class>

    <owl:Class rdf:about="http://purl.org/metam#Category">
        <rdfs:label>Category</rdfs:label>
        <rdfs:comment></rdfs:comment>
        <rdfs:subClassOf rdf:resource="http://purl.org/metam#ClassificationConcept"/>
    </owl:Class>

    <owl:Class rdf:about="http://purl.org/metam#Class">
        <rdfs:label>Class</rdfs:label>
        <rdfs:comment></rdfs:comment>
        <rdfs:subClassOf rdf:resource="http://purl.org/metam#ClassificationConcept"/>
    </owl:Class>

    <owl:Class rdf:about="http://purl.org/metam#Condition">
        <rdfs:label>Condition</rdfs:label>
        <rdfs:comment></rdfs:comment>
        <rdfs:subClassOf rdf:resource="http://purl.org/metam#ClassificationConcept"/>
    </owl:Class>

    <owl:Class rdf:about="http://purl.org/metam#Trait">
        <rdfs:label>Trait</rdfs:label>
        <rdfs:comment></rdfs:comment>
        <rdfs:subClassOf rdf:resource="http://purl.org/metam#DescriptiveConcept"/>
    </owl:Class>

    <owl:Class rdf:about="http://purl.org/metam#PsychopathologicalCategory">
        <rdfs:label>Psychopathological Category</rdfs:label>
        <rdfs:comment>A class representing broad groups of psychopathological features used for the classification and diagnosis of mental disorders. These categories can be subdivided into different levels (e.g., Superspectra, Spectra) to describe various dimensions and severities of mental disorders.</rdfs:comment>
        <rdfs:subClassOf rdf:resource="http://purl.org/metam#Category"/>
    </owl:Class>

    <owl:Class rdf:about="http://purl.org/metam#PsychopathologicalClass">
        <rdfs:label>Psychopathological Class</rdfs:label>
        <rdfs:comment>A fundamental class within a psychopathological category that represents specific features or dimensions of a mental disorder. Psychopathological Elements are the building blocks used for detailed description and analysis of subfactors and symptoms.</rdfs:comment>
        <rdfs:subClassOf rdf:resource="http://purl.org/metam#Class"/>
    </owl:Class>

    <owl:Class rdf:about="http://purl.org/metam#PathologicalCondition">
        <rdfs:label>Pathological Condition</rdfs:label>
        <rdfs:comment>A class of conditions representing physical or mental deviations from normal health. Pathological Conditions include both physical and mental disorders, characterized by specific symptoms and features.</rdfs:comment>
        <rdfs:subClassOf rdf:resource="http://purl.org/metam#Condition"/>
    </owl:Class>

    <owl:Class rdf:about="http://purl.org/metam#PsychologicalTrait">
        <rdfs:label>Psychological Trait</rdfs:label>
        <rdfs:comment>A class of qualities representing stable, enduring characteristics of an individual's psychological state. These qualities influence behavior, perception, and emotional experience and can appear as traits within psychopathological taxonomies.</rdfs:comment>
        <rdfs:subClassOf rdf:resource="http://purl.org/metam#Quality"/>
    </owl:Class>

    <owl:Class rdf:about="http://purl.org/metam#PathologicalTrait">
        <rdfs:label>Pathological Trait</rdfs:label>
        <rdfs:comment>A class of qualities representing specific signs or symptoms of a Pathological Condition. These qualities manifest as observable or experienced deviations from normal function and serve as indicators of the presence of a disease or disorder.</rdfs:comment>
        <rdfs:subClassOf rdf:resource="http://purl.org/metam#Trait"/>
    </owl:Class>

    <!-- Define the Superspectra class as a subclass of PsychopathologicalCategory -->
    <owl:Class rdf:about="http://purl.org/htp#Superspectra">
        <rdfs:subClassOf rdf:resource="http://purl.org/metam#PsychopathologicalCategory"/>
    </owl:Class>

    <!-- Define the Component class as a subclass of PsychopathologicalClass -->
    <owl:Class rdf:about="http://purl.org/htp#Component">
        <rdfs:subClassOf rdf:resource="http://purl.org/metam#PsychopathologicalClass"/>
    </owl:Class>

    <!-- Define the Disorder class as a subclass of PathologicalCondition -->
    <owl:Class rdf:about="http://purl.org/htp#Disorder">
        <rdfs:subClassOf rdf:resource="http://purl.org/metam#PathologicalCondition"/>
    </owl:Class>

    <!-- Define the Trait class as a subclass of PsychologicalTrait -->
    <owl:Class rdf:about="http://purl.org/htp#Trait">
        <rdfs:subClassOf rdf:resource="http://purl.org/metam#PsychologicalTrait"/>
    </owl:Class>

    <!-- Define the Symptom class as a subclass of PathologicalTrait -->
    <owl:Class rdf:about="http://purl.org/htp#Symptom">
        <rdfs:subClassOf rdf:resource="http://purl.org/metam#PathologicalTrait"/>
    </owl:Class>

    <!-- Importing BFO -->
    <owl:imports rdf:resource="http://purl.obolibrary.org/obo/bfo.owl"/>

    <!-- Importing HiTOP -->
    <owl:imports rdf:resource="http://purl.org/htp#"/>

    <!-- Represents an ontology module within the meta-ontology framework. -->
    <!-- Includes properties for versioning, licensing, and compliance with BFO. -->
    <owl:Class rdf:about="metam:OntologyModule">
        <rdfs:label>Ontology Module</rdfs:label>
        <rdfs:comment>A modular part of an ontology to facilitate integration.</rdfs:comment>
        <rdfs:subClassOf rdf:resource="http://www.w3.org/2002/07/owl#Thing"/>
    </owl:Class>

    <!-- A rule that defines how concepts from different ontologies are mapped to facilitate integration. -->
    <!-- This class can be used to specify how elements from one ontology correspond to elements in another ontology. -->
    <owl:Class rdf:about="meta:MappingRule">
        <rdfs:label>Mapping Rule</rdfs:label>
        <rdfs:comment>A rule that defines how concepts from different ontologies are mapped.</rdfs:comment>
    </owl:Class>

    <!-- Indicates that one concept is a temporal refinement or specialization of another concept. -->
    <!-- This relationship pertains to time-bound events or processes. -->
    <owl:ObjectProperty rdf:about="meta:isTemporalRefinementOf">
        <rdfs:label>Temporal Refinement Of</rdfs:label>
        <rdfs:comment>Indicates that one concept is a temporal refinement or specialization of another concept, where the refinement is related to time-bound events or processes.</rdfs:comment>
        <rdfs:domain rdf:resource="bfo:Occurent"/>
        <rdfs:range rdf:resource="bfo:Occurent"/>
    </owl:ObjectProperty>

    <!-- Indicates that one concept is a temporal generalization or broader category of another concept. -->
    <!-- This relationship pertains to time-bound events or processes. -->
    <owl:ObjectProperty rdf:about="meta:isTemporalGeneralizationOf">
        <rdfs:label>Temporal Generalization Of</rdfs:label>
        <rdfs:comment>Indicates that one concept is a temporal generalization or broader category of another concept, where the generalization is related to time-bound events or processes.</rdfs:comment>
        <rdfs:domain rdf:resource="bfo:Occurent"/>
        <rdfs:range rdf:resource="bfo:Occurent"/>
    </owl:ObjectProperty>

    <!-- Indicates that one concept is a constant refinement or specialization of another concept. -->
    <!-- Both concepts are considered constant over time. -->
    <owl:ObjectProperty rdf:about="meta:isConstantRefinementOf">
        <rdfs:label>Constant Refinement Of</rdfs:label>
        <rdfs:comment>Indicates that one concept is a constant refinement or specialization of another concept, where both concepts are considered constant over time.</rdfs:comment>
        <rdfs:domain rdf:resource="bfo:Continuant"/>
        <rdfs:range rdf:resource="bfo:Continuant"/>
    </owl:ObjectProperty>

    <!-- Indicates that one concept is a constant generalization or broader category of another concept. -->
    <!-- Both concepts are considered constant over time. -->
    <owl:ObjectProperty rdf:about="meta:isConstantGeneralizationOf">
        <rdfs:label>Constant Generalization Of</rdfs:label>
        <rdfs:comment>Indicates that one concept is a constant generalization or broader category of another concept, where both concepts are considered constant over time.</rdfs:comment>
        <rdfs:domain rdf:resource="bfo:Continuant"/>
        <rdfs:range rdf:resource="bfo:Continuant"/>
    </owl:ObjectProperty>

    <!-- The domain or field that the ontology module is relevant to (e.g., medicine, biology). -->
    <!-- Specifies the primary area of application for the ontology module. -->
    <owl:DatatypeProperty rdf:about="metam:hasDomain">
        <rdfs:label>Domain</rdfs:label>
        <rdfs:comment>The domain or field that the ontology module is relevant to (e.g., medicine, biology).</rdfs:comment>
        <rdfs:domain rdf:resource="metam:OntologyModule"/>
        <rdfs:range rdf:resource="xsd:string"/>
    </owl:DatatypeProperty>

    <!-- Indicates whether the ontology module is compliant with the Basic Formal Ontology (BFO). -->
    <!-- This helps in verifying if the module adheres to BFO standards for ontology integration. -->
    <owl:DatatypeProperty rdf:about="metam:isBFOCompliant">
        <rdfs:label>BFO Compliant</rdfs:label>
        <rdfs:comment>This property indicates whether the ontology module is compliant with the Basic Formal Ontology (BFO).</rdfs:comment>
        <rdfs:domain rdf:resource="metam:OntologyModule"/>
        <rdfs:range rdf:resource="xsd:boolean"/>
    </owl:DatatypeProperty>

    <!-- The scope of the ontology module. -->
    <!-- Indicates whether the coverage is broad or specific. -->
    <owl:DatatypeProperty rdf:about="metam:scope">
        <rdfs:label>Scope</rdfs:label>
        <rdfs:comment>The scope of the ontology module (e.g., broad or specific coverage).</rdfs:comment>
        <rdfs:domain rdf:resource="metam:OntologyModule"/>
        <rdfs:range rdf:resource="xsd:string"/>
    </owl:DatatypeProperty>

    <!-- Specifies potential use cases for the ontology module. -->
    <!-- Describes the practical applications or scenarios where the ontology can be utilized. -->
    <owl:DatatypeProperty rdf:about="metam:useCase">
        <rdfs:label>Use Case</rdfs:label>
        <rdfs:comment>Specifies potential use cases for the ontology module.</rdfs:comment>
        <rdfs:domain rdf:resource="metam:OntologyModule"/>
        <rdfs:range rdf:resource="xsd:string"/>
    </owl:DatatypeProperty>

    <!-- Indicates which systems or ontologies use this module. -->
    <!-- Specifies the relationships between the ontology module and other modules or systems that rely on it. -->
    <owl:ObjectProperty rdf:about="metam:isUsedBy">
        <rdfs:label>Is Used By</rdfs:label>
        <rdfs:comment>Indicates which systems or ontologies use this module.</rdfs:comment>
        <rdfs:domain rdf:resource="metam:OntologyModule"/>
        <rdfs:range rdf:resource="metam:OntologyModule"/>
    </owl:ObjectProperty>

</rdf:RDF>